Cslib/Foundations/Data/StackTape.lean
@@ -85,16 +85,16 @@ def cons (x : Option Symbol) (xs : StackTape Symbol) : StackTape Symbol :=
   | none, ⟨hd :: tl, hl⟩ => ⟨none :: hd :: tl, by grind⟩
   | some a, ⟨l, hl⟩ => ⟨some a :: l, by grind⟩
 
-@[simp, scoped grind =]
+@[simp]
 lemma cons_none_nil_toList : (cons none (nil : StackTape Symbol)).toList = [] := by grind
 
-@[simp, scoped grind =]
+@[simp]
 lemma cons_none_nil : cons none (nil : StackTape Symbol) = nil := rfl
 
-@[simp, scoped grind =]
+@[simp]
 lemma cons_none_empty : cons none (∅ : StackTape Symbol) = ∅ := rfl
 
-@[simp, scoped grind =]
+@[simp]
 lemma cons_some_toList (a : Symbol) (l : StackTape Symbol) :
     (cons (some a) l).toList = some a :: l.toList := by simp only [cons]
 
@@ -136,7 +136,9 @@ lemma head_cons (o : Option Symbol) (l : StackTape Symbol) : (cons o l).head = o
   | none =>
     cases l with | mk toList hl =>
     cases toList <;> grind
-  | some a => grind
+  | some a =>
+    cases l with | mk toList hl =>
+    simp [cons, head]
 
 @[simp]
 lemma tail_cons (o : Option Symbol) (l : StackTape Symbol) : (cons o l).tail = l := by
@@ -204,7 +206,8 @@ lemma length_cons_none (l : StackTape Symbol) :
 @[scoped grind =]
 lemma length_cons_some (a : Symbol) (l : StackTape Symbol) :
     (cons (some a) l).length = l.length + 1 := by
-  grind
+  cases l with | mk toList hl =>
+  simp [length, cons]
 
 lemma length_cons_le (o : Option Symbol) (l : StackTape Symbol) :
     (cons o l).length ≤ l.length + 1 := by
